Finish 1st impl of state and actions

tryf/Quint.State.fst
@@ -1,70 +1,251 @@
 
+
 module Quint.State
 
 open Quint.Util
 
 module DM = FStar.DependentMap
+module List = FStar.List.Tot
+open List
 
-//// START dep map try
-noeq
-type sig =
-  { vars: eqtype
-  ; vals: vars -> Type
-  }
+class sig = {
+   /// `vars` is the set of "flexible variables"
+   vars:eqtype;
+   /// `types` maps each variable to the types of the values it can be assigned
+   types: vars -> Type
+}
 
-let state (s:sig) = DM.t s.vars s.vals
-
-type var =
-  | V
-  | X
-
-let var_type : var -> Type = function
-  | V -> int
-  | X -> string
-
-let optional : (var -> Type) -> var -> Type =
+let optional #k : (k -> Type) -> k -> Type =
   fun f v -> option (f v)
 
-let s = state {vars = var; vals = optional var_type}
 
-let init_t : Type = v:var -> var_type v
+let state {| sig |} = DM.t vars (optional types)
 
-let init : init_t = function
-  | V -> 0
-  | X -> "foo"
+let is_assigned {| sig |} (m:state) k = Some? (DM.sel m k)
+let is_unassigned {| sig |} (m:state) k = None? (DM.sel m k)
 
-let init_opt: f:(v:var -> var_type v) -> v':var -> option (var_type v') =
+let is_fresh {| sig |} (m:state) = forall k. is_unassigned m k
+
+let is_updated {| sig |} (m:state) = forall k. is_assigned m k
+
+let init_opt {| sig |}: f:(v:vars -> types v) -> v':vars -> option (types v') =
   fun init variable -> Some (init variable)
 
-let is_fresh (m:s) = forall k. None? (DM.sel m k)
-let is_updated (m:s) = forall k. Some? (DM.sel m k)
+type init_t {| sig |} = v:vars -> types v
 
-let upd (v:var) (x:var_type v)
-  : m:s{None? (DM.sel m v)} -> m':s{Some? (DM.sel m' v)} =
-  fun m -> DM.upd m v (Some x)
+let init (s:sig) (f:init_t) : state = DM.create (init_opt f)
 
-
-let initial_state (f:init_t) : s = DM.create (init_opt f)
-let empty_state : m:s{is_fresh m} =
+let empty_state {| sig |} : m:state{is_fresh m} =
   let clear _ = None in
   DM.create (clear)
+
+let upd {| sig |} (v:vars) (x:types v)
+  : m:state{is_unassigned m v} -> m':state{is_assigned m' v} =
+  fun m -> DM.upd m v (Some x)
+
+// let ( := ) {|sig|} = upd
+
+let transition {| sig |} = s0:state{is_updated s0} -> s1:state{is_updated s1}
+
+// START State Example
+type ex_var = | V | X
+instance ex_sig : sig = {
+  vars = ex_var;
+  types = function
+    | V -> int
+    | X -> string
+}
 
 // Trying to update the same variable twice fails
 [@@expect_failure [54]]
 let _ex_cannot_update_twice = (~(upd V 1 empty_state |> upd V 10))
 
-let _ex_is_updated_empty = assert_norm (~(is_updated empty_state))
+let _ex_is_updated_empty = assert_norm (~(is_updated (empty_state)))
 let _ex_is_updated_partial = assert_norm (~(is_updated (empty_state |> upd V 1)))
 let _ex_is_updated = assert_norm (is_updated ( upd V 1  empty_state |> upd X "foo" ))
 
-let m = initial_state init
-let init_ex = assert (is_updated m)
-let v_ex = assert_norm (DM.sel m V = Some 0)
-let x_ex = assert_norm (DM.sel m X = Some "foo")
-//// END dep map try
+let _s = init ex_sig (function
+  | V -> 0
+  | X -> "foo")
 
+let _ex_init = assert_norm (is_updated _s)
+let _ex_v = assert_norm (DM.sel _s V = Some 0)
+let _ex_x = assert_norm (DM.sel _s X = Some "foo")
+
+// let _ex_acess_state = assert_norm (V@_s = 0 && X@_s = "foo")
+// let _ex_set_state : state =
+//     (V := 5) empty_state |> (X := "fee")
+// END State Example
+
+// TODO Use `DM.restrict` to limit map to just declared variables
+// A computation of `a` that can read from `state #sig`
+
+let state_has {|sig|} (s:state) (vs:list vars) =
+    forall v. mem v vs ==> is_assigned s v
+
+let state_not_has {|sig|} (s:state) (vs:list vars) =
+    forall v. mem v vs ==> is_unassigned s v
+
+// Copied from  https://github.com/shonfeder/FStar/tree/fd0f8db6e8e254a51f0c872067004cd83d3a1f5e/ulib/FStar.List.Tot.Properties.fst
+// which has the SMTPat commented out
+val append_mem: #t:eqtype ->  l1:list t
+              -> l2:list t
+              -> a:t
+              -> Lemma (requires True)
+                       (ensures (mem a (l1@l2) = (mem a l1 || mem a l2)))
+                       [SMTPat (mem a (l1@l2))]
+let rec append_mem #t l1 l2 a = match l1 with
+  | [] -> ()
+  | hd::tl -> append_mem tl l2 a
+
+let state_concat_has_both {|sig|} (vs vs': list vars) (s:state{state_has s (vs @ vs')})
+    : Lemma (state_has s vs /\ state_has s vs')
+    = ()
+
+let state_concat_is_concat_ls {|sig|} (vss vs vs': list vars) (s:state)
+    : Lemma (vss == vs @ vs' ==> state_has s vss == state_has s (vs @ vs'))
+    = ()
+
+// let rec state_concat_has_both {|sig|}
+//  (vs vs':list vars) (s:state)
+//  : Lemma (state_has s (vs @ vs') ==> state_has s vs /\ state_has s vs')
+//  = match vs with
+//  | [] -> List.append_nil_l vs'; assert (state_has s vs')
+//  | x :: xs -> assert (is_assigned s x); state_concat_has_both xs vs'
+
+// let state_has_both {|sig|} (s:state) vs vs' =
+//  state_has s vs && state_has s vs'
+
+/// the type of computations that
+///
+/// - read from a state with signature `sig`
+/// - read the variables in `vs` (so all `v` in `vs` must be assigned)
+/// - produces a vlue of type `a`
+type read {|sig|} (vs:list vars) (a:Type)
+  = s:state{state_has s vs} -> a
+
+let read_map {|sig|} #a #b #vs (f:a -> b) (x:read vs a) : read vs b
+  = fun s -> f (x s)
+
+let return {|sig|} #a (x:a) : read [] a = fun _ -> x
+
+let (let@) {|sig|} #a #b #vs
+  (x : read vs a) (f : a -> read vs b) : read vs b
+  = fun s -> f (x s) s
+
+let (and@) {|sig|} #a #b #vs #vs'
+  (x : read vs a) (y : read vs' b) : read (vs @ vs') (a * b)
+  = fun s -> (x s, y s)
+
+let ( ! ) {| sig |} (v:vars) : read [v] (types v) // s:state{is_assigned s v} -> types v
+    =
+    fun state -> Some?.v (DM.sel state v)
+
+let read_ex : read [X; V] (int * string) =
+    let@ x = !V
+    and@ v = !X
+    in
+    return (x, v)
+
+type action_vars {|sig|} = {
+  updated : list vars;
+  updates : list vars;
+  not_updated : list vars;
+  }
+
+/// A state predicate, i.e., an action
+///
+/// - `s0` is the current state
+/// - `s` is the intermediate state to be updated (lets us ensure no state is updated twice)
+/// - `s1` is the next state specified by by the action
+type action_t {|sig|} (vs:list vars)
+  = s0:state{is_updated s0}
+    -> option (
+      s:state{state_not_has s vs}
+      -> s1:state{state_has s1 vs /\ (forall v. (not (mem v vs)) ==> DM.sel s1 v == DM.sel s v)}
+    )
+
+// /// A state predicate, i.e., an action
+// ///
+// /// - `s0` is the current state
+// /// - `s` is the intermediate state to be updated (lets us ensure no state is updated twice)
+// /// - `s1` is the next state specified by by the action
+// type action_t {|sig|} (vs:action_vars)
+//   = s0:state -> option (s:state{state_has s vs.updated /\ state_not_has s (vs.updates @ vs.not_updated)} -> s1:state{state_has s1 (vs.updated @ vs.updates) /\ state_not_has s1 vs.not_updated})
+
+// let upd' {| sig |} (v:vars) (x:types v) updated not_updated
+//   : s:state{state_has s updated /\ state_not_has s ([v] @ not_updated)} -> s':state{state_has s ([v] @ updated) /\ state_not_has s not_updated} =
+//   fun m -> DM.upd m v (Some x)
+
+let ( @= ) {|sig|} (v:vars) (x:types v) : action_t [v]
+  = fun _ -> Some (fun s -> upd v x s)
+
+/// Conjunction is the composition of actions
+let ( &! ) {|sig|} #vs #vs'
+  (a1:action_t vs)
+  (a2:action_t vs'{forall v. mem v vs' ==> not (mem v vs)}) // a2 cannot update the same vars as a1
+  : action_t (vs @ vs') // ther
+  =
+  fun s0 ->
+  match a1 s0 with
+  | None -> None
+  | Some upd1 ->
+  match a2 s0 with
+  | None -> None
+  | Some upd2 ->
+  Some (fun (s:state{state_not_has s (vs @ vs')}) -> (upd2 (upd1 s)))
+
+// TODO Add non-det
+let ( |! ) {|sig|} #vs (a1:action_t vs) (a2:action_t vs) : action_t vs  =
+  fun s0 ->
+  match a1 s0 with
+  | Some upd1 -> Some upd1
+  | None ->
+  a2 s0
+
+// TODO: need to adjust precedence so don't need to use brackets
+let _ex_conj : action_t [V; X] =
+  (  V @= 1
+  &! X @= "foo"
+  )
+
+let _ex_disj : action_t [V] =
+  (  V @= 1
+  |! V @= 2
+  )
+
+let _ex_comb : action_t [V; X] =
+  (  V @= 1
+  &! X @= "foo"
+  )
+  |!
+  (  V @= 10
+  &! X @= "fee"
+  )
+
+
+
+// let all {|sig|} : action j -> state -> option state =
+
+// Like return, but we don't have values to return
+let enact {|sig|} : action = fun s -> [], s
+
+let (let!) {|sig|} #a
+  (x: action) (f: action)
+  : action
+  = fun s ->
+    let cs, s' = x s in
+    let cs', s'' = f s' in
+    (cs @ cs', s'')
+
+
+
+// TODO: Add support for _next_ state
+// TODO: A monad that will build up a series of constraints (requirements) and a state_update.
+// A transition is enabled if all the constraints
 // TODO: Add a boolean to state, indicating whether the action was enabled,
 // TODO: State is actual relating this state and next state, updates go to next state, reads from this state
+
 type time a =
   { trace: list a
   ; t0 : a
